intersections and unions

BourbakiLean2/Set/Operations.lean
@@ -1,1 +1,254 @@
 import BourbakiLean2.Function.Basic
+import Batteries
+import Batteries.Util.ExtendedBinder
+variable {α β : Type*} {ι ι' : Type*} {x : ι → Set α} {y : ι → Set β} {a : α} {i : ι}
+
+namespace Set
+def iUnion (x : ι → Set α) := {a | ∃ i, a ∈ x i}
+def iInter (x : ι → Set α) := {a | ∀ i, a ∈ x i}
+section
+open Lean Elab Term Meta Batteries.ExtendedBinder
+syntax (name := iUnionBuilder) "⋃ " extBinder ", " term:51 : term
+@[term_elab iUnionBuilder]
+def elabiUnionBuilder : TermElab
+  | `(⋃ $x:ident , $p ), expectedType? => do
+    elabTerm (← `(iUnion fun $x:ident ↦ $p)) expectedType?
+  | `(⋃ $x:ident : $t , $p ), expectedType? => do
+    elabTerm (← `(iUnion fun $x:ident : $t ↦ $p)) expectedType?
+  | `(⋃ $x:ident $b:binderPred , $p ), expectedType? => do
+    elabTerm (← `(iUnion fun $x:ident ↦ satisfies_binder_pred% $x $b ∧ $p)) expectedType?
+  | _, _ => throwUnsupportedSyntax
+
+/-- Unexpander for set builder notation. -/
+@[app_unexpander iUnion]
+def iUnion.unexpander : Lean.PrettyPrinter.Unexpander
+  | `($_ fun $x:ident ↦ $p) => `(⋃ $x:ident , $p )
+  | `($_ fun ($x:ident : $ty:term) ↦ $p) => `(⋃ $x:ident : $ty , $p )
+  | _ => throw ()
+
+syntax (name := iInterBuilder) "⋂ " extBinder ", " term:51 : term
+@[term_elab iInterBuilder]
+def elabiInterBuilder : TermElab
+  | `(⋂ $x:ident , $p ), expectedType? => do
+    elabTerm (← `(iInter fun $x:ident ↦ $p)) expectedType?
+  | `(⋂ $x:ident : $t , $p ), expectedType? => do
+    elabTerm (← `(iInter fun $x:ident : $t ↦ $p)) expectedType?
+  | `(⋂ $x:ident $b:binderPred , $p ), expectedType? => do
+    elabTerm (← `(iInter fun $x:ident ↦ satisfies_binder_pred% $x $b ∧ $p)) expectedType?
+  | _, _ => throwUnsupportedSyntax
+
+/-- Unexpander for set builder notation. -/
+@[app_unexpander iInter]
+def iInter.unexpander : Lean.PrettyPrinter.Unexpander
+  | `($_ fun $x:ident ↦ $p) => `(⋂ $x:ident , $p )
+  | `($_ fun ($x:ident : $ty:term) ↦ $p) => `(⋂ $x:ident : $ty , $p )
+  | _ => throw ()
+
+end
+
+@[simp] theorem mem_iUnion_iff : a ∈ ⋃ i, x i ↔ ∃i, a ∈ x i := Iff.rfl
+theorem mem_iUnion_of (h : a ∈ x i) : a ∈ ⋃ i, x i := mem_iUnion_iff.mpr ⟨_,h⟩
+theorem of_mem_iUnion (h : a ∈ ⋃ i, x i) : ∃ i, a ∈ x i := mem_iUnion_iff.mp h
+@[simp] theorem subset_iUnion : x i ⊆ ⋃ i, x i := fun _ => mem_iUnion_of
+
+@[simp] theorem iUnion_subset_iff_all {y : Set α} : ⋃ i, x i ⊆ y ↔ ∀i, x i ⊆ y := by
+  constructor
+  · intro h i
+    trans ⋃ i, x i
+    · exact subset_iUnion
+    · exact h
+  · rintro h a ⟨i,h'⟩
+    exact h _ h'
+
+theorem iUnion_empty_index (h : ι → False) : ⋃ i, x i = ∅ := by
+  rw[← subset_empty_iff]
+  rintro i ⟨w,_⟩
+  exact h w
+
+@[simp] theorem iUnion_empty_iff : ⋃ i, x i = ∅ ↔ ∀ i, x i = ∅ := by
+  constructor
+  · intro h i
+    rw[← subset_empty_iff, ← h]
+    simp only [subset_iUnion]
+  · rw[← subset_empty_iff]
+    rintro h a ⟨i,h'⟩
+    simp only [h i, not_mem_empty] at h'
+
+@[simp] theorem mem_iInter_iff : a ∈ ⋂ i, x i ↔ ∀i, a ∈ x i := Iff.rfl
+theorem mem_iInter_of (h : ∀i, a ∈ x i) : a ∈ ⋂ i, x i := mem_iInter_iff.mpr h
+theorem of_mem_iInter (h : a ∈ ⋂ i, x i) : a ∈ x i := mem_iInter_iff.mp h i
+
+@[simp] theorem iInter_subset : ⋂ i, x i ⊆ x i := fun _ => of_mem_iInter
+
+@[simp] theorem subset_iInter_iff_all {y : Set α} : y ⊆ ⋂ i, x i ↔ ∀ i, y ⊆ x i := by
+  constructor
+  · intro h i a h'
+    exact iInter_subset (h h')
+  · intro h a h' i
+    exact h i h'
+
+theorem iInter_empty_index (h : ι → False) : ⋂ i, x i = Set.univ := by
+  ext a
+  simp only [mem_iInter_iff, mem_univ, iff_true]
+  intro i
+  exact (h i).elim
+
+@[simp] theorem iInter_univ_iff : ⋂ i, x i = Set.univ ↔ ∀ i, x i = Set.univ := by
+  constructor
+  · intro h i
+    rw[← univ_subset_iff, ← h]
+    simp only [iInter_subset]
+  · rw[← univ_subset_iff]
+    rintro h a _ i
+    simp only [h i, mem_univ]
+
+@[simp] theorem iUnion_singleton {x : Unit → Set α} : ⋃ i, x i = x ⟨⟩ := by
+  ext a
+  constructor
+  · rintro ⟨⟨⟩,h⟩
+    exact h
+  · rintro h
+    exact ⟨⟨⟩,h⟩
+
+@[simp] theorem iInter_singleton {x : Unit → Set α} : ⋂ i, x i = x ⟨⟩ := by
+  ext a
+  constructor
+  · intro h
+    exact h ⟨⟩
+  · rintro h ⟨⟩
+    exact h
+
+theorem iUnion_index_change_subset {f : ι' → ι} : ⋃ i', x (f i') ⊆ ⋃ i, x i := by
+  intro a
+  simp only [mem_iUnion_iff]
+  rintro ⟨i', h'⟩
+  exact ⟨f i',h'⟩
+
+theorem iUnion_index_change_surj {f : ι' → ι}  (h : f.Surjective) : ⋃ i', x (f i') = ⋃ i, x i := by
+  ext a
+  simp only [mem_iUnion_iff]
+  constructor
+  apply iUnion_index_change_subset
+  · rintro ⟨i, h'⟩
+    obtain ⟨_,rfl⟩ := h.exists_preimage i
+    exact ⟨_,h'⟩
+
+theorem iInter_subset_index_change {f : ι' → ι} : ⋂ i, x i ⊆ ⋂ i', x (f i') := by
+  intro a h i'
+  simp only [mem_iInter_iff]
+  exact h (f i')
+
+theorem iInter_index_change_surj {f : ι' → ι} (h : f.Surjective) : ⋂ i', x (f i') = ⋂ i, x i := by
+  ext a
+  constructor
+  · rintro h' i
+    simp only [mem_iInter_iff]
+    obtain ⟨_,rfl⟩ := h.exists_preimage i
+    apply h'
+  · apply iInter_subset_index_change
+
+theorem iUnion_constant (h : ∀ i i', x i = x i') : ⋃ i, x i = x i := by
+  ext a
+  simp
+  constructor
+  · rintro ⟨i',h'⟩
+    rw[h] at h'
+    exact h'
+  · apply Exists.intro i
+
+theorem iInter_constant (h : ∀ i i', x i = x i') : ⋂ i, x i = x i := by
+  ext a
+  simp
+  constructor
+  · intro h'
+    exact h' i
+  · intro h' i'
+    rw[h _ i'] at h'
+    exact h'
+
+
+theorem iUnion_index_mono {p : ι → Prop} : ⋃ i : {i // p i}, x i ⊆ ⋃ i, x i := by
+  rintro a ⟨⟨i,h⟩,h'⟩
+  exists i
+
+theorem iInter_index_mono {p : ι → Prop} : ⋂ i, x i ⊆ ⋂ i : {i // p i}, x i := by
+  rintro a h ⟨i,h'⟩
+  apply_assumption
+
+theorem iInter_subset_iUnion [Nonempty ι] : ⋂ i, x i ⊆ ⋃ i, x i := by
+  intro a h
+  exists Classical.choice (by infer_instance)
+  apply h
+
+section
+variable {x' : ι → Set α}
+
+theorem iUnion_mono (h : ∀ i, x i ⊆ x' i) : ⋃ i, x i ⊆ ⋃ i, x' i := by
+  rw[iUnion_subset_iff_all]
+  intro i
+  exact subset_trans (h i) subset_iUnion
+
+theorem iInter_mono (h : ∀ i, x i ⊆ x' i) : ⋂ i, x i ⊆ ⋂ i, x' i := by
+  rw[subset_iInter_iff_all]
+  intro i
+  exact subset_trans iInter_subset (h i)
+end
+
+theorem iUnion_assoc {x : ι → ι' → Set α} : ⋃ i : ι × ι', x i.1 i.2 = ⋃ j, (⋃ i, x j i) := by
+  ext a
+  simp only [mem_iUnion_iff, Prod.exists]
+
+theorem iInter_assoc {x : ι → ι' → Set α} : ⋂ i : ι × ι', x i.1 i.2 = ⋂ j, (⋂ i, x j i) := by
+  ext a
+  simp only [mem_iInter_iff, Prod.forall]
+
+end Set
+
+section
+variable {r : Relation α β}
+
+theorem Relation.iUnion_image : r.image (⋃ i, x i) = ⋃ i, r.image (x i) := by
+  ext a
+  simp only [Relation.mem_image_iff, Set.mem_iUnion_iff]
+  rw[exists_comm]
+  apply exists_congr
+  intro a'
+  simp only [exists_and_left]
+
+theorem Relation.iUnion_preimage : r.preimage (⋃ i, y i) = ⋃ i, r.preimage (y i) := by
+  rw[← r.image_inv]
+  conv =>
+    rhs
+    rhs
+    intro i
+    rw[← r.image_inv]
+  apply iUnion_image
+
+theorem Relation.subset_iInter_image : r.image (⋂ i, x i) ⊆ ⋂ i, r.image (x i) := by
+  intro b ⟨a',h, h'⟩
+  intro i
+  simp at *
+  exact ⟨_,h,h' _⟩
+
+theorem Relation.subset_iInter_preimage : r.preimage (⋂ i, y i) ⊆ ⋂ i, r.preimage (y i) := by
+  intro b ⟨a',h, h'⟩
+  intro i
+  simp at *
+  exact ⟨_,h,h' _⟩
+end
+
+section
+variable {f : α → β}
+theorem Set.iUnion_image : Set.image f (⋃ i, x i) = ⋃ i, Set.image f (x i) := Relation.iUnion_image
+theorem Set.iUnion_preimage : Set.preimage f (⋃ i, y i) = ⋃ i, Set.preimage f (y i) := Relation.iUnion_preimage
+theorem Set.subset_iInter_image : Set.image f (⋂ i, x i) ⊆ ⋂ i, Set.image f (x i) := Relation.subset_iInter_image
+theorem Set.iInter_preimage : Set.preimage f (⋂ i, y i) = ⋂ i, Set.preimage f (y i) := by
+  apply subset_antisym
+  · apply Relation.subset_iInter_preimage
+  · intro a h
+    simp only [mem_iInter_iff, mem_preimage_iff] at h
+    simpa only [mem_preimage_iff, mem_iInter_iff] using h
+
+
+
+end
